swotarfe_andufotions/src/PropL.v
@@ -596,7 +596,7 @@ Qed.
 (* Exercise: 2 stars (total_relation) *)
 
 Inductive total_relation : nat -> nat -> Prop :=
-  | tr : forall n m, total_relation n m.
+  | tot : forall n m, total_relation n m.
 
 (* END total_relation. *)
 
